# Analytical Exercise 1.2

by Qiang Gao, updated at May 17, 2017

## Chapter 1 Finite-Sample Properties of OLS

...

### Analytical Exercise 1.2 \(The annihilator associated with the vector of ones\)

Let $$\mathbf{1}$$ be the $$n$$-dimensional column vector of ones, and let $$\mathbf{M}_1 \equiv \mathbf{I}_n - \mathbf{1} ( \mathbf{1}' \mathbf{1} )^{-1} \mathbf{1}'$$. That is, $$\mathbf{M}_1$$ is the annihilator associated with $$\mathbf{1}$$. Prove the following:

\(a\) $$\mathbf{M}_1$$ is symmetric and idempotent.

\(b\) $$\mathbf{M}_1 \mathbf{1} = \mathbf{0}$$.

\(c\) $$\mathbf{M}_1 \mathbf{y} = \mathbf{y} - \bar{y} \cdot \mathbf{1}$$ where

$$
\bar{y} = \frac{1}{n} \sum_{i=1}^{n} y_i.
$$

$$\mathbf{M}_1 \mathbf{y}$$ is the vector of **deviations from the mean**.

#### Solution

\(a\) The symmetry of $$\mathbf{M}_1$$ is verified as

$$
\begin{align}
\mathbf{M}'_1 & = \mathbf{I}'_n - ( \mathbf{1} ( \mathbf{1}' \mathbf{1} )^{-1} \mathbf{1}' )'
\\ & =
\mathbf{I}_n - \mathbf{1} ( \mathbf{1}' \mathbf{1} )^{-1} \mathbf{1}'
&& \text{(Because 
$( \mathbf{A} \mathbf{B} )' = \mathbf{B}' \mathbf{A}' $,
$ ( \mathbf{A}^{-1} )' = ( \mathbf{A}' )^{-1} $)}
\\ & =
\mathbf{M}_1.
\end{align}
$$

The idempotency of $$\mathbf{M}_1$$ is verified as

$$
\begin{align}
\mathbf{M}_1 \mathbf{M}_1 & = ( \mathbf{I}_n - \mathbf{1} ( \mathbf{1}' \mathbf{1} )^{-1} \mathbf{1}' )( \mathbf{I}_n - \mathbf{1} ( \mathbf{1}' \mathbf{1} )^{-1} \mathbf{1}' )
\\ & =
\mathbf{I}_n
- \mathbf{1} ( \mathbf{1}' \mathbf{1} )^{-1} \mathbf{1}'
- \mathbf{1} ( \mathbf{1}' \mathbf{1} )^{-1} \mathbf{1}'
+ \mathbf{1} ( \mathbf{1}' \mathbf{1} )^{-1} \mathbf{1}'
\mathbf{1} ( \mathbf{1}' \mathbf{1} )^{-1} \mathbf{1}'
\\ & =
\mathbf{I}_n
- \mathbf{1} ( \mathbf{1}' \mathbf{1} )^{-1} \mathbf{1}'
- \mathbf{1} ( \mathbf{1}' \mathbf{1} )^{-1} \mathbf{1}'
+ \mathbf{1} ( \mathbf{1}' \mathbf{1} )^{-1} \mathbf{1}'
\\ & =
\mathbf{I}_n
- \mathbf{1} ( \mathbf{1}' \mathbf{1} )^{-1} \mathbf{1}'
\\ & =
\mathbf{M}_1.
\end{align}
$$

\(b\)

$$
\begin{align}
\mathbf{M}_1 \mathbf{1} & =
( \mathbf{I}_n - \mathbf{1} ( \mathbf{1}' \mathbf{1} )^{-1} \mathbf{1}' ) \mathbf{1}
\\ & =
\mathbf{1} - \mathbf{1} ( \mathbf{1}' \mathbf{1} )^{-1} \mathbf{1}' \mathbf{1}
\\ & =
\mathbf{1} - \mathbf{1}
\\ & =
\mathbf{0}.
\end{align}
$$

\(c\)

$$
\begin{align}
\mathbf{M}_{1} \mathbf{y} & = ( \mathbf{I}_n - \mathbf{1} ( \mathbf{1}' \mathbf{1} )^{-1} \mathbf{1}' ) \mathbf{y}
\\ & =
\mathbf{y} - \mathbf{1} ( \mathbf{1}' \mathbf{1} )^{-1} \mathbf{1}' \mathbf{y}
\\ & =
\mathbf{y} - \mathbf{1} \cdot \frac{1}{n} \cdot \sum_{i=1}^{n} y_i
\\ & =
\mathbf{y} - \bar{y} \cdot \mathbf{1}.
\end{align}
$$

Copyright Â©2017 by Qiang Gao

