# Review Question 2.1.2

by Qiang Gao, updated at June 8, 2018

## Chapter 2 Large-Sample Theory

### Section 1 Review of Limit Theorems for Sequences of Random Variables

...

#### Review Question 2.1.2 \(Alternative definition of convergence for vector sequences\)

\(a\) Verify that the definition in the text of “$$\mathbf{z}_n \to_{m.s.} \mathbf{z}$$” is equivalent to

$$
\lim_{n \to \infty} \operatorname{E}
[ ( \mathbf{z}_n - \mathbf{z} )'( \mathbf{z}_n - \mathbf{z} ) ]
= 0.
$$

**Hint**: $$\operatorname{E} [ ( \mathbf{z}_n - \mathbf{z} )'( \mathbf{z}_n - \mathbf{z} ) ] = \operatorname{E} [ ( z_{n1} - z_1 )^2 ] + \cdots + \operatorname{E} [ ( z_{nK} - z_K )^2 ]$$, where $$K$$ is the dimension of $$\mathbf{z}$$.

\(b\) Similarly, verify that the definition in the text of “$$\mathbf{z}_n \to_p \boldsymbol{\alpha}$$” is equivalent to

$$
\lim_{n \to \infty} \operatorname{Prob}
\left(
( \mathbf{z}_n - \boldsymbol{\alpha} )'
( \mathbf{z}_n - \boldsymbol{\alpha} ) >
\varepsilon
\right) = 0,
$$

for any $$\varepsilon > 0$$.

**Solution**

\(a\) If $$\mathbf{z}_n \to_{m.s.} \mathbf{z}$$, by definition in the text,

$$
\lim_{n \to \infty} \operatorname{E}
[ ( z_{nk} - z_k )^2 ] = 0,
\text{ for $k = 1, \ldots, K$},
$$

then we can show

$$
\begin{align}
& \color{white}{=} \lim_{n \to \infty} \operatorname{E}
[ ( \mathbf{z}_n - \mathbf{z} )'( \mathbf{z}_n - \mathbf{z} ) ] \\
& = \lim_{n \to \infty}
\left(
\operatorname{E} [ ( z_{n1} - z_1 )^2 ] + \cdots + 
\operatorname{E} [ ( z_{nK} - z_K )^2 ]
\right) \\
& = \lim_{n \to \infty} \operatorname{E} [ ( z_{n1} - z_1 )^2 ] + \cdots + 
\lim_{n \to \infty} \operatorname{E} [ ( z_{nK} - z_K )^2 ] \\
& = 0.
\end{align}
$$

If $$\lim_{n \to \infty} \operatorname{E} [ ( \mathbf{z}_n - \mathbf{z} )'( \mathbf{z}_n - \mathbf{z} ) ] = 0$$, then

$$
\lim_{n \to \infty} \operatorname{E} [ ( z_{n1} - z_1 )^2 ] + \cdots + 
\lim_{n \to \infty} \operatorname{E} [ ( z_{nK} - z_K )^2 ] = 0.
\tag{1}
$$

Because each terms in \(1\) are non-negative, \(1\) implies

$$
\lim_{n \to \infty} \operatorname{E}
[ ( z_{nk} - z_k )^2 ] = 0,
\text{ for $k = 1, \ldots, K$},
$$

which means $$z_{nk} \to_{m.s.} z_k$$ for $$k = 1, \ldots, K$$, and this implies $$\mathbf{z}_n \to_{m.s.} \mathbf{z}$$ by definition in the text.

\(b\) Similarly, if $$\mathbf{z}_n \to_p \boldsymbol{\alpha}$$, by definition in the text, for any $$\varepsilon > 0$$,

$$
\operatorname{Prob}
\left(
| z_{nk} - \alpha_k | > \varepsilon
\right) \to 0,
\text{ for $k = 1, \ldots, K$},
$$

then we can show

$$
\begin{gather}
\operatorname{Prob}
\left(
( z_{nk} - \alpha_k )^2 > \varepsilon^2
\right) \to 0,
\text{ for $k = 1, \ldots, K$}, 
&& \text{(equivalent event)} \\

\operatorname{Prob}
\left(
( z_{nk} - \alpha_k )^2 > \varepsilon
\right) \to 0,
\text{ for $k = 1, \ldots, K$},
&& \text{(any $\varepsilon > 0$)} \\

\operatorname{Prob}
\left(
( z_{n1} - \alpha_1 )^2 > \varepsilon
\right) + \cdots +
\operatorname{Prob}
\left(
( z_{nK} - \alpha_K )^2 > \varepsilon
\right) \to 0, 
&& \text{(limit sum)} \\

\left(
\not\Rightarrow
\operatorname{Prob}
\left(
(z_{n1} - \alpha_1)^2 + \cdots + (z_{nK} - \alpha_K)^2 > K \varepsilon
\right) \to 0
\right)
&& \text{(bigger event)} \\

\operatorname{Prob}
\left(
\bigcup_{k=1}^K
\left(
( z_{nk} - \alpha_k )^2 > \varepsilon
\right)
\right) \to 0, 
&& \text{(smaller event)} \\

\operatorname{Prob}
\left(
\bigcap_{k=1}^K
\left(
( z_{nk} - \alpha_k )^2 \leq \varepsilon
\right)
\right) \to 1, 
&& \text{(complement event)} \\

\operatorname{Prob}
\left(
( z_{n1} - \alpha_1 )^2 + \cdots +
( z_{nK} - \alpha_K )^2 \leq K \varepsilon
\right) \to 1, 
&& \text{(bigger event)} \\

\operatorname{Prob}
\left(
( z_{n1} - \alpha_1 )^2 + \cdots +
( z_{nK} - \alpha_K )^2 \leq \varepsilon
\right) \to 1,
&& \text{(any $\varepsilon > 0$)} \\

\operatorname{Prob}
\left(
( \mathbf{z}_n - \boldsymbol{\alpha} )'
( \mathbf{z}_n - \boldsymbol{\alpha} )
\leq \varepsilon
\right) \to 1, 
&& \text{(matrix notation)} \\

\operatorname{Prob}
\left(
( \mathbf{z}_n - \boldsymbol{\alpha} )'
( \mathbf{z}_n - \boldsymbol{\alpha} )
> \varepsilon
\right) \to 0.
&& \text{(complement event)}
\end{gather}
$$

If $$\operatorname{Prob} \left( ( \mathbf{z}_n - \boldsymbol{\alpha} )' ( \mathbf{z}_n - \boldsymbol{\alpha} ) > \varepsilon \right) \to 0$$, then we can show

$$
\begin{gather}
\operatorname{Prob}
\left(
( z_{n1} - \alpha_1 )^2 + \cdots +
( z_{nK} - \alpha_K )^2 > \varepsilon
\right) \to 0, 
&& \text{(scalar notation)} \\

\operatorname{Prob}
\left(
\bigcup_{k=1}^K
\left(
( z_{nk} - \alpha_k )^2 > \varepsilon
\right)
\right) \to 0, 
&& \text{(smaller event)} \\

\operatorname{Prob}
\left(
( z_{nk} - \alpha_k )^2 > \varepsilon
\right) \to 0
\text{ for $k = 1, \ldots, K$ },
&& \text{(smaller events)}
\end{gather}
$$

which means $$z_{nk} \to_p \alpha_k$$ for $$k = 1, \ldots, K$$, and this implies $$\mathbf{z}_n \to_p \boldsymbol{\alpha}$$.

Copyright ©2018 by Qiang Gao

