# Review Question 1.2.9

by Qiang Gao, updated at Mar 26, 2017

## Chapter 1 Finite-Sample Properties of OLS

### Section 2 The Algebra of Least Squares

...

#### Review Question 1.2.9 \(Computation of the statistics\)

Verify that $$\mathbf{b}$$, $$\mathrm{SSR}$$, $$s^2$$, and $$R^2$$ can be calculated from the following sample averages: $$\mathbf{S}_{ \mathbf{x} \mathbf{x} }$$, $$\mathbf{s}_{ \mathbf{x} \mathbf{y} }$$, $$\mathbf{y}' \mathbf{y} / n$$, and $$\bar{y}$$. \(If the regressors include a constant, then $$\bar{y}$$ is the element of $$\mathbf{s}_{ \mathbf{x} \mathbf{y} }$$ corresponding to the constant.\) Therefore, those sample averages need to be computed just once in order to obtain the regression coefficients and related statistics.

**Solution**

\(1\) According to \(1.2.5'\),

$$
\mathbf{b} = \mathbf{S}_{\mathbf{x} \mathbf{x}}^{-1}
\mathbf{s}_{\mathbf{x} \mathbf{y}}.
$$

\(2\)

$$
\begin{align}
\mathrm{SSR} & = \mathbf{e}' \mathbf{e}
&&
\text{(definition (1.2.12))}
\\ & = 
(\mathbf{y} - \mathbf{X} \mathbf{b})'
(\mathbf{y} - \mathbf{X} \mathbf{b})
&&
\text{(definition (1.2.4))}
\\ & =
\mathbf{y}'\mathbf{y} - \mathbf{y}' \mathbf{X}
\mathbf{b} - \mathbf{b}' \mathbf{X}' \mathbf{y} +
\mathbf{b}' \mathbf{X}' \mathbf{X} \mathbf{b}
\\ & =
\mathbf{y}'\mathbf{y} - \mathbf{y}' \mathbf{X}
\mathbf{b} - \mathbf{b}' \mathbf{X}' \mathbf{y} +
\mathbf{b}' \mathbf{X}' \mathbf{y}
&&
\text{(definition (1.2.5))}
\\ & =
\mathbf{y}'\mathbf{y} - (\mathbf{X}' \mathbf{y})' \mathbf{b}
\\ & =
n \cdot \mathbf{y}' \mathbf{y} / n - n \cdot
\mathbf{s}_{\mathbf{x} \mathbf{y}}'
\mathbf{S}_{\mathbf{x} \mathbf{x}}^{-1}
\mathbf{s}_{\mathbf{x} \mathbf{y}}
\\ & =
n \cdot ( \mathbf{y}' \mathbf{y} / n -
\mathbf{s}_{\mathbf{x} \mathbf{y}}'
\mathbf{S}_{\mathbf{x} \mathbf{x}}^{-1}
\mathbf{s}_{\mathbf{x} \mathbf{y}} ).  
\end{align}
$$

\(3\)

$$
s^2 = \frac{\mathrm{SSR}}{n - K} = 
\frac{n}{n - K} \cdot ( \mathbf{y}' \mathbf{y} / n -
\mathbf{s}_{\mathbf{x} \mathbf{y}}'
\mathbf{S}_{\mathbf{x} \mathbf{x}}^{-1}
\mathbf{s}_{\mathbf{x} \mathbf{y}} ).
$$

\(4\)

$$
\begin{align}
R^2 & = 1 - \frac{ \mathrm{SSR} }
{ \sum_{i=1}^n (y_i - \bar{y})^2 }
&&
\text{(definition (1.2.18))}
\\ & =
1 - \frac{ \mathrm{SSR} }
{ \sum_{i=1}^n (y_i^2 - 2\bar{y}y_i + \bar{y}^2) }
\\ & =
1 - \frac{ \mathrm{SSR} }
{ \sum_{i=1}^n y_i^2 - 2 \bar{y} \sum_{i=1}^n y_i +
\sum_{i=1}^n \bar{y}^2 }
\\ & =
1 - \frac{ \mathrm{SSR} }
{ n \cdot \mathbf{y}' \mathbf{y} / n -
2n \cdot \bar{y}^2 + n \cdot \bar{y}^2}
\\ & =
1 - \frac{ \mathrm{SSR} }
{ n \cdot \mathbf{y}' \mathbf{y} / n -
n \cdot \bar{y}^2}.
\end{align}
$$

Copyright Â©2017 by Qiang Gao

