# Review Question 1.2.5

by Qiang Gao, updated at Mar 21, 2017

## Chapter 1 Finite-Sample Properties of OLS

### Section 2 The Algebra of Least Squares

...

#### Review Question 1.2.5 \(Matrix algebra of fitted values and residuals\)

Show the following:

\(a\) $$\hat{\mathbf{y}} = \mathbf{P} \mathbf{y}$$, $$\mathbf{e} = \mathbf{M} \mathbf{y} = \mathbf{M} \boldsymbol{\varepsilon}$$.

\(b\) $$\mathrm{SSR} = \boldsymbol{\varepsilon}' \mathbf{M} \boldsymbol{\varepsilon}$$.

**Solution**

\(a.1\) $$\hat{\mathbf{y}} = \mathbf{P} \mathbf{y}$$ because

$$
\begin{align}
\hat{\mathbf{y}}
& =
\mathbf{X} \mathbf{b}
&&
\text{(definition of $\hat{\mathbf{y}}$)}
\\ & =
\mathbf{X} ( \mathbf{X}' \mathbf{X} )^{-1} \mathbf{X}' \mathbf{y}
&&
\text{(definition of $\mathbf{b}$)}
\\ & =
\mathbf{P} \mathbf{y}.
&&
\text{(definition of $\mathbf{P}$)}
\end{align}
$$

\(a.2\) $$\mathbf{e} = \mathbf{M} \mathbf{y} = \mathbf{M} \boldsymbol{\varepsilon}$$ because

$$
\begin{align}
\mathbf{e} & = \mathbf{y} - \mathbf{X} \mathbf{b}
&&
\text{(definition of $\mathbf{e}$)}
\\ & =
\mathbf{y} - \hat{\mathbf{y}}
&&
\text{(definition of $\hat{\mathbf{y}}$)}
\\ & =
\mathbf{y} - \mathbf{P} \mathbf{y}
&&
(\hat{\mathbf{y}} = \mathbf{P} \mathbf{y})
\\ & =
(\mathbf{I} - \mathbf{P}) \mathbf{y}
\\ & =
\mathbf{M} \mathbf{y}
&&
\text{(definition of $\mathbf{M}$)}
\\ & =
\mathbf{M} ( \mathbf{X} \boldsymbol{\beta} + \boldsymbol{ \varepsilon } )
&&
\text{(Assumption 1.1)}
\\ & =
\mathbf{M} \mathbf{X} \boldsymbol{\beta} +
\mathbf{M} \boldsymbol{\varepsilon}
\\ & =
\mathbf{M} \boldsymbol{\varepsilon}
&&
(\mathbf{M} \mathbf{X} = \mathbf{0})
\end{align}
$$

\(b\) $$\mathrm{SSR} = \boldsymbol{\varepsilon}' \mathbf{M} \boldsymbol{\varepsilon}$$ because

$$
\begin{align}
\mathrm{SSR} & = \mathbf{e}' \mathbf{e}
&&
\text{(definition of $\mathrm{SSR}$)}
\\ & =
(\mathbf{M} \boldsymbol{\varepsilon})'
(\mathbf{M} \boldsymbol{\varepsilon})
&&
( \mathbf{e} = \mathbf{M} \boldsymbol{\varepsilon} )
\\ & =
\boldsymbol{\varepsilon}' \mathbf{M} \mathbf{M}
\boldsymbol{\varepsilon}
\\ & =
\boldsymbol{\varepsilon}' \mathbf{M}
\boldsymbol{\varepsilon}.
&&
\text{($\mathbf{M}$ is idempotent)}
\end{align}
$$

Copyright Â©2017 by Qiang Gao

